coq: set theory

coq/set/Core/Compatible.v
@@ -8,27 +8,30 @@ Require Import Core.Semantics.
 Require Import Core.Environment.
 
 Definition compatible (P:set -> Prop) : Prop :=
-    forall (x y:set), x == y -> P x -> P y.
+    forall (x x':set), x == x' -> P x -> P x'.
+
+Definition compatible2 (P:set -> set -> Prop) : Prop :=
+    forall (x x' y y':set), x == x' -> y == y' -> P x y -> P x' y'.
 
 (* Any predicate obtained by a formula is a compatible predicate.               *)
-Theorem formulaCompatible : forall (e:Env) (n:nat) (p:Formula),
-    compatible (eval' e n p). 
+Theorem formulaCompatible : forall (e:Env) (p:Formula) (n:nat),
+    compatible (eval1 e p n). 
 Proof.
-    intros e n p. revert e n. induction p as [|k m|p1 IH1 p2 IH2|m p1 IH1];
-    intros e n; unfold compatible, eval'; intros x y E; simpl; intros H.
+    intros e p n. revert e n. induction p as [|k m|p1 IH1 p2 IH2|m p1 IH1];
+    intros e n; unfold compatible, eval1; intros x y E; simpl; intros H.
     - assumption.
     - apply equal_l with (bind e n x k). 
         + apply bindEqual. assumption.
         + apply equal_r with (bind e n x m).
             { apply bindEqual. assumption. }
             { assumption. }
-    - unfold compatible, eval' in IH1. unfold compatible, eval' in IH2. intros H'.
+    - unfold compatible, eval1 in IH1. unfold compatible, eval1 in IH2. intros H'.
       apply IH2 with x.
         + assumption.
         + apply H. apply IH1 with y.
             { apply equalSym. assumption. }
             { assumption. }
-    - intros z. unfold compatible, eval' in IH1. 
+    - intros z. unfold compatible, eval1 in IH1. 
       destruct (eq_nat_dec m n) as [H'|H'].
         + subst. apply (evalEnvEqual (bind (bind e n y) n z) (bind e n z)).
             { apply bindOver. }
@@ -47,3 +50,18 @@ Proof.
                     { apply bindPermute. assumption. }
                     { apply H. }}}
 Qed.
+
+(*
+(* Any two-fold predicate obtained by a formula is a compatible predicate.      *)
+Theorem formulaCompatible2 : forall (e:Env) (p:Formula) (n m:nat),
+    compatible2 (eval2 e p n m).
+Proof.
+    unfold eval2. intros e p n m x x' y y' Hx Hy H.
+    remember (formulaCompatible (bind e n x') p m) as H' eqn:E. clear E.
+    unfold compatible in H'. unfold eval1 in H'. apply H' with y; clear H'.
+    - assumption.
+    - 
+
+
+Show.
+*)
